src/Compiler.fst
@@ -1,0 +1,300 @@
+(** Main compiler transformation *)
+module Compiler
+
+(* Reversible circuit interpretation -- compiles a Revs program
+   to a reversible circuit in a "natural" way. Specifically, 
+   the circuit reflects the structure of the program *)
+type circState =
+  { top : int;
+    ah : AncHeap;
+    gates : list Gate;
+    subs : Total.t int int }
+
+val circInit   : circState
+val circAlloc  : circState -> BoolExp -> Tot (int * circState)
+val circAssign : circState -> int -> BoolExp -> Tot circState
+val circEval   : circState -> state -> int -> Tot bool
+
+let circInit = {top = 0; ah = emptyHeap; gates = []; subs = constMap 0}
+let circAlloc cs bexp =
+  let (ah', res, ancs, circ') = compileBexp_oop cs.ah (substVar bexp cs.subs) in
+  let top' = cs.top + 1 in
+  let gates' = cs.gates @ circ' in
+  let subs' = update cs.subs cs.top res in
+  (cs.top, {top = top'; ah = ah'; gates = gates'; subs = subs'})
+let circAssign cs l bexp =
+  let l' = lookup cs.subs l in
+  let bexp' = substVar bexp cs.subs in
+  let (ah', res, ancs, circ') = match factorAs bexp' l' with
+    | None -> compileBexp_oop cs.ah bexp'
+    | Some bexp'' -> compileBexp cs.ah l' bexp''
+  in
+  {top = cs.top; ah = ah'; gates = cs.gates @ circ'; subs = update cs.subs l res}
+let circEval cs ivals i = lookup (evalCirc cs.gates ivals) (lookup cs.subs i)
+
+let circInterp = {
+  alloc = circAlloc;
+  assign = circAssign;
+  eval = circEval
+}
+
+val allocNcirc : list GExpr * circState -> i:int ->
+  Tot (list GExpr * circState) (decreases i)
+let rec allocNcirc (locs, cs) i =
+  if i <= 0 then (List.rev locs, cs)
+  else
+    let (ah', res) = popMin cs.ah in
+    let cs' = { top = cs.top + 1;
+                ah = ah';
+                gates = cs.gates;
+                subs = update cs.subs cs.top res }
+    in
+      allocNcirc (((LOC cs.top)::locs), cs') (i-1)
+
+val allocTycirc : GType -> circState -> Tot (result (GExpr * circState))
+let allocTycirc ty cs = match ty with
+  | GBool ->
+    let (ah', res) = popMin cs.ah in
+    let cs' = { top = cs.top + 1;
+                ah = ah';
+                gates = cs.gates;
+                subs = update cs.subs cs.top res }
+    in
+      Val (LOC cs.top, cs')
+  | GArray n ->
+    let (locs, st') = allocNcirc ([], cs) n in
+      Val (ARRAY locs, st')
+  | _ -> Err "Invalid parameter type for circuit generation"
+
+val lookup_Lst : st:Total.t int int -> lst:(list GExpr){isVal_lst lst} -> Tot (list int)
+let rec lookup_Lst st lst = match lst with
+  | [] -> []
+  | (LOC l)::xs -> (lookup st l)::(lookup_Lst st xs)
+
+val compileCirc : config circState -> Dv (result (list int * list Gate))
+let rec compileCirc (gexp, cs) =
+  if isVal gexp then match gexp with
+    | UNIT -> Val ([], [])
+    | LAMBDA (x, ty, t) ->
+      begin match allocTycirc ty cs with
+        | Err s -> Err s
+        | Val (v, cs') -> compileCirc (substGExpr t x v, cs')
+      end
+    | LOC l ->
+      let res = lookup cs.subs l in
+        Val ([res], cs.gates)
+    | ARRAY lst ->
+      let res = lookup_Lst cs.subs lst in
+        Val (res, cs.gates)
+  else match (step (gexp, cs) circInterp) with
+    | Err s -> Err s
+    | Val c' -> compileCirc c'
+
+(** Verification utilities *)
+(* Correctness of circuit compilation *)
+type circ_equiv (st:boolState) (cs:circState) (init:state) =
+  fst st = cs.top /\
+  zeroHeap (evalCirc cs.gates init) cs.ah /\
+  (forall i. not (mem (lookup cs.subs i) cs.ah)) /\
+  (forall i. boolEval st init i = circEval cs init i)
+
+(* Needed for disjointness after applying substitution *)
+val substVar_disjoint : bexp:BoolExp -> subs:Total.t int int -> s:set int ->
+  Lemma (requires (forall i. not (Set.mem (lookup subs i) s)))
+        (ensures  (disjoint s (vars (substVar bexp subs))))
+let rec substVar_disjoint bexp subs s = match bexp with
+  | BFalse -> ()
+  | BVar i -> ()
+  | BNot x -> substVar_disjoint x subs s
+  | BAnd (x, y) | BXor (x, y) -> 
+    substVar_disjoint x subs s; 
+    substVar_disjoint y subs s
+
+val eval_bexp_swap2 : st:boolState -> cs:circState -> bexp:BoolExp -> bexp':BoolExp -> init:state ->
+  Lemma (requires (circ_equiv st cs init /\
+                   bexp' = substVar bexp cs.subs /\
+                   disjoint (elts cs.ah) (vars bexp')))
+        (ensures  (evalBexp bexp (snd st) = evalBexp bexp' (evalCirc cs.gates init)))
+let rec eval_bexp_swap2 st cs bexp bexp' init = match (bexp, bexp') with
+  | (BFalse, _) -> ()
+  | (BVar i, _) -> ()
+  | (BNot x, BNot x') -> eval_bexp_swap2 st cs x x' init
+  | (BAnd (x, y), BAnd (x', y')) | (BXor (x, y), (BXor (x', y'))) ->
+    eval_bexp_swap2 st cs x x' init;
+    eval_bexp_swap2 st cs y y' init
+
+val eval_commutes_subst_circ : st:boolState -> cs:circState -> bexp:BoolExp ->
+  bexp':BoolExp -> init:state -> targ:int -> targ':int ->
+  Lemma (requires (circ_equiv st cs init /\
+                   bexp' = substVar bexp cs.subs /\
+                   targ' = lookup cs.subs targ /\
+                   not (Set.mem targ' (vars bexp')) /\
+                   not (Set.mem targ' (elts cs.ah)) /\
+                   disjoint (elts cs.ah) (vars bexp')))
+        (ensures  (lookup (evalCirc (last (compileBexp cs.ah targ' bexp'))
+                                    (evalCirc cs.gates init)) targ' 
+                   =
+                   lookup (snd st) targ <> evalBexp bexp (snd st)))
+let eval_commutes_subst_circ st cs bexp bexp' init targ targ' =
+  let init' = evalCirc cs.gates init in
+    compile_bexp_correct cs.ah targ' bexp' init';
+    eval_bexp_swap2 st cs bexp bexp' init
+
+val eval_commutes_subst_circ_oop : st:boolState -> cs:circState ->
+  bexp:BoolExp -> bexp':BoolExp -> init:state ->
+  Lemma (requires (circ_equiv st cs init /\
+                   bexp' = substVar bexp cs.subs /\
+                   disjoint (elts cs.ah) (vars bexp')))
+        (ensures  (lookup (evalCirc (last (compileBexp_oop cs.ah bexp'))
+                                    (evalCirc cs.gates init))
+                          (second (compileBexp_oop cs.ah bexp')) 
+                   = evalBexp bexp (snd st)))
+let eval_commutes_subst_circ_oop st cs bexp bexp' init =
+  let init' = evalCirc cs.gates init in
+    compile_bexp_correct_oop cs.ah bexp' init';
+    eval_bexp_swap2 st cs bexp bexp' init
+
+val circ_equiv_alloc : st:boolState -> cs:circState -> init:state -> bexp:BoolExp ->
+  Lemma (requires (circ_equiv st cs init))
+        (ensures  (circ_equiv (snd (boolAlloc st bexp)) (snd (circAlloc cs bexp)) init))
+let circ_equiv_alloc st cs init bexp =
+  let bexp' = substVar bexp cs.subs in
+  let init' = evalCirc cs.gates init in
+  let (ah', res, ancs, circ') = compileBexp_oop cs.ah bexp' in
+  let st' = snd (boolAlloc st bexp) in
+  let cs' = snd (circAlloc cs bexp) in
+  let zeroHeap_lem =
+    substVar_disjoint bexp cs.subs (elts cs.ah);
+    compile_decreases_heap_oop cs.ah bexp';
+    compile_partition_oop cs.ah bexp';
+    zeroHeap_subset init' cs.ah cs'.ah;
+    zeroHeap_st_impl init' cs'.ah circ'
+  in
+  let preservation =
+    compile_mods_oop cs.ah bexp';
+    eval_mod init' circ'
+  in
+  let correctness =
+    eval_commutes_subst_circ_oop st cs bexp bexp' init
+  in
+  ()
+
+val circ_equiv_assign : st:boolState -> cs:circState -> init:state -> l:int -> bexp:BoolExp ->
+  Lemma (requires (circ_equiv st cs init))
+        (ensures  (circ_equiv (boolAssign st l bexp) (circAssign cs l bexp) init))
+let circ_equiv_assign st cs init l bexp =
+  let l' = lookup cs.subs l in
+  let bexp' = substVar bexp cs.subs in
+  let init' = evalCirc cs.gates init in
+  let st' = boolAssign st l bexp in
+  let cs' = circAssign cs l bexp in
+  match factorAs bexp' l' with
+    | None ->
+      let (ah', res, ancs, circ') = compileBexp_oop cs.ah bexp' in
+      let zeroHeap_lem =
+        substVar_disjoint bexp cs.subs (elts cs.ah);
+        compile_decreases_heap_oop cs.ah bexp';
+        compile_partition_oop cs.ah bexp';
+        zeroHeap_subset init' cs.ah cs'.ah;
+        zeroHeap_st_impl init' cs'.ah circ'
+      in
+      let preservation =
+        compile_mods_oop cs.ah bexp';
+        eval_mod init' circ'
+      in
+      let correctness =
+        eval_commutes_subst_circ_oop st cs bexp bexp' init
+      in
+      ()
+    | Some bexp'' -> (* TODO: Fix this, doesn't pass anymore *)
+      let (ah', res, ancs, circ') = compileBexp cs.ah l' bexp'' in
+      let zeroHeap_lem =
+        factorAs_correct bexp' l' init';
+        factorAs_vars bexp' l';
+        substVar_disjoint bexp cs.subs (elts cs.ah);
+        disjoint_subset (vars bexp'') (vars bexp') (elts cs.ah);
+        compile_decreases_heap cs.ah l' bexp'';
+        compile_partition cs.ah l' bexp'';
+        zeroHeap_subset init' cs.ah cs'.ah;
+        zeroHeap_st_impl init' cs'.ah circ'
+      in
+      let preservation = //admitP(forall i. not (i = l) ==> boolEval st' init i = circEval cs' init i);
+        compile_mods cs.ah l' bexp'';
+        eval_mod init' circ'
+      in
+      let correctness = //admitP(b2t(lookup (snd st') l = lookup (evalCirc circ' init') (lookup cs'.subs l)))
+        admitP(b2t(boolEval st' init l = circEval cs' init l));
+        eval_commutes_subst_circ st cs bexp bexp'' init l l'
+      in
+        //admitP(forall i. boolEval st' init i = circEval cs' init i);
+      ()
+
+
+(* TODO: Fix this, doesn't pass anymore *)
+val circ_equiv_step : gexp:GExpr -> st:boolState -> st':circState -> init:state ->
+  Lemma (requires (circ_equiv st st' init))
+        (ensures
+          (is_Err (step (gexp, st) boolInterp) /\ is_Err (step (gexp, st') circInterp)) \/
+          (is_Val (step (gexp, st) boolInterp) /\ is_Val (step (gexp, st') circInterp) /\
+          (fst (getVal (step (gexp, st) boolInterp)) =
+           fst (getVal (step (gexp, st') circInterp)) /\
+          circ_equiv (snd (getVal (step (gexp, st) boolInterp)))
+                      (snd (getVal (step (gexp, st') circInterp)))
+                      init)))
+  (decreases %[gexp;1])
+val circ_equiv_step_lst : lst:list GExpr -> st:boolState -> st':circState -> init:state ->
+  Lemma (requires (circ_equiv st st' init))
+        (ensures
+          (is_Err (step_lst (lst, st) boolInterp) /\ is_Err (step_lst (lst, st') circInterp)) \/
+          (is_Val (step_lst (lst, st) boolInterp) /\ is_Val (step_lst (lst, st') circInterp) /\
+          (fst (getVal (step_lst (lst, st) boolInterp)) =
+           fst (getVal (step_lst (lst, st') circInterp)) /\
+          circ_equiv (snd (getVal (step_lst (lst, st) boolInterp)))
+                      (snd (getVal (step_lst (lst, st') circInterp)))
+                      init)))
+  (decreases %[lst;0])
+let rec circ_equiv_step gexp st st' init = match gexp with
+  | LET (x, t1, t2) ->
+    circ_equiv_step t1 st st' init
+  | LAMBDA (x, ty, t) -> ()
+  | APPLY (t1, t2) ->
+    circ_equiv_step t1 st st' init;
+    circ_equiv_step t2 st st' init
+  | SEQUENCE (t1, t2) ->
+    circ_equiv_step t1 st st' init;
+    circ_equiv_step t2 st st' init
+  | ASSIGN (t1, t2) ->
+    circ_equiv_step t1 st st' init;
+    circ_equiv_step t2 st st' init;
+    if (isVal t1 && isBexp t2) then
+      begin match t1 with
+        | LOC l -> circ_equiv_assign st st' init l (get_bexp t2)
+        | _ -> ()
+      end
+  | XOR (t1, t2) ->
+    circ_equiv_step t1 st st' init;
+    circ_equiv_step t2 st st' init
+  | AND (t1, t2) ->
+    circ_equiv_step t1 st st' init;
+    circ_equiv_step t2 st st' init
+  | BOOL b -> ()
+  | APPEND (t1, t2) ->
+    circ_equiv_step t1 st st' init;
+    circ_equiv_step t2 st st' init
+  | ROT (i, t) ->
+    circ_equiv_step t st st' init
+  | SLICE (t, i, j) ->
+    circ_equiv_step t st st' init
+  | ARRAY lst ->
+    circ_equiv_step_lst lst st st' init
+  | GET_ARRAY (t, i) ->
+    circ_equiv_step t st st' init
+  | ASSERT t ->
+    circ_equiv_step t st st' init
+  | BEXP bexp -> circ_equiv_alloc st st' init bexp
+  | _ -> ()
+and circ_equiv_step_lst lst st st' init = match lst with
+  | [] -> ()
+  | x::xs ->
+    circ_equiv_step x st st' init;
+    circ_equiv_step_lst xs st st' init
