src/Crush.fst
@@ -1,0 +1,233 @@
+(** Program transformation/compiler based on minimal ESOP forms *)
+module Crush
+
+open Util
+open Total
+open BoolExp
+open ExprTypes
+open Interpreter
+
+(* Boolean expression interpretation -- for generating the fully
+   inlined classical circuit of the Revs program *)
+type BExpState = int * (Total.t int BoolExp)
+
+val bexpInit   : BExpState
+val bexpAlloc  : BExpState -> BoolExp -> Tot (int * BExpState)
+val bexpAssign : BExpState -> int -> BoolExp -> Tot BExpState
+val bexpEval   : BExpState -> state -> int -> Tot bool
+
+let bexpInit = (0, constMap BFalse)
+let bexpAlloc (top, st) bexp =
+  (top, (top + 1, update st top (substBexp bexp st)))
+let bexpAssign (top, st) l bexp =
+  (top, update st l (substBexp bexp st))
+let bexpEval (top, st) ivals i = evalBexp (lookup st i) ivals
+
+let bexpInterp = {
+  alloc = bexpAlloc;
+  assign = bexpAssign;
+  eval = bexpEval
+}
+
+type CleanupStrategy =
+  | Pebbled : CleanupStrategy
+  | Boundaries : CleanupStrategy
+  | Bennett : CleanupStrategy
+
+val simps : BoolExp -> Tot BoolExp
+let simps bexp = simplify (toXDNF bexp)
+
+val allocN : list GExpr * BExpState -> i:int ->
+  Tot (list GExpr * BExpState) (decreases i)
+let rec allocN (locs, (top, st)) i =
+  if i <= 0 then (List.rev locs, (top, st))
+  else allocN (((LOC top)::locs), (top+1, update st top (BVar top))) (i-1)
+
+val allocTy : GType -> BExpState -> Tot (result (GExpr * BExpState))
+let allocTy ty (top, st) = match ty with
+  | GBool -> Val (LOC top, (top + 1, update st top (BVar top)))
+  | GArray n ->
+    let (locs, st') = allocN ([], (top, st)) n in
+      Val (ARRAY locs, st')
+  | _ -> Err "Invalid parameter type for circuit generation"
+
+val lookupLst : lst:(list GExpr){isVal_lst lst} -> st:BExpState -> Tot (list BoolExp)
+let rec lookupLst lst st = match lst with
+  | [] -> []
+  | (LOC l)::xs -> (lookup (snd st) l)::(lookupLst xs st)
+
+open AncillaHeap
+open Circuit
+
+val foldPebble : (AncHeap * list int * list int * list Gate) ->
+  BoolExp -> Tot (AncHeap * list int * list int * list Gate)
+let foldPebble (ah, outs, anc, circ) bexp =
+  let (ah', res, anc', circ') = compileBexpPebbled_oop ah (simps bexp) in
+    (ah', res::outs, anc'@anc, circ@circ')
+
+val foldClean : (AncHeap * list int * list int * list Gate) ->
+  BoolExp -> Tot (AncHeap * list int * list int * list Gate)
+let foldClean (ah, outs, anc, circ) bexp =
+  let (ah', res, anc', circ') = compileBexpClean_oop ah (simps bexp) in
+    (ah', res::outs, anc'@anc, circ@circ')
+
+val foldBennett : (AncHeap * list int * list int * list Gate * list Gate) ->
+  BoolExp -> Tot (AncHeap * list int * list int * list Gate * list Gate)
+let foldBennett (ah, outs, anc, circ, ucirc) bexp =
+  let (ah', res, anc', circ') = compileBexp_oop ah (simps bexp) in
+    (ah', res::outs, anc'@anc, circ@circ', (List.rev (uncompute circ' res))@ucirc)
+
+(* Compilation wrapper. The main point of interest is its action when the
+   program is a function. In that case it allocates some new free variables
+   corresponding to the inputs of the function, then evaluates the function
+   body. Note also that this wrapper is not verified currently. Eventually this
+   should be done. *)
+val compile : config BExpState -> CleanupStrategy -> Dv (result (list int * list Gate))
+let rec compile (gexp, st) strategy =
+  if isVal gexp then match gexp with
+    | UNIT -> Val ([], [])
+    | LAMBDA (x, ty, t) ->
+      begin match allocTy ty st with
+        | Err s -> Err s
+        | Val (v, st') -> compile (substGExpr t x v, st') strategy
+      end
+    | LOC l ->
+      let bexp = lookup (snd st) l in
+      let max = varMax bexp in
+      let (ah, res, anc, circ) = match strategy with
+        | Pebbled -> compileBexpPebbled_oop (above (max+1)) (simps bexp)
+        | Boundaries -> compileBexpClean_oop (above (max+1)) (simps bexp)
+        | Bennett -> compileBexpClean_oop (above (max+1)) (simps bexp)
+      in
+        Val ([res], circ)
+    | ARRAY lst ->
+      let cmp x y = 
+	let xd = andDepth x in
+	let yd = andDepth y in
+	  if xd < yd then 1 else if xd = yd then 0 else -1
+      in
+      let blst = List.sortWithT cmp (lookupLst lst st) in
+      let max = listMax (List.mapT varMax blst) in
+      let (ah, outs, anc, circ) = match strategy with
+        | Pebbled ->
+          let (ah, outs, anc, circ) =
+            List.fold_leftT foldPebble (above (max+1), [], [], []) blst
+          in
+            (ah, List.rev outs, List.rev anc, circ)
+        | Boundaries ->
+          let (ah, outs, anc, circ) =
+            List.fold_leftT foldClean (above (max+1), [], [], []) blst
+          in
+            (ah, List.rev outs, List.rev anc, circ)
+        | Bennett ->
+          let (ah, outs, anc, circ, ucirc) =
+            List.fold_leftT foldBennett (above (max+1), [], [], [], []) blst
+          in
+            (ah, List.rev outs, List.rev anc, circ@ucirc)
+      in
+        Val (outs, circ)
+  else match (step (gexp, st) bexpInterp) with
+    | Err s -> Err s
+    | Val c' -> compile c' strategy
+
+(** Verification utilities *)
+(* Originally this was done polymorphically (using a general notion of
+   equivalence of states and a proof that the interpreter preserves equivalence
+   if alloc and assign do). Eventually this should be refactored that way, but
+   this was faster for the time being. *)
+type state_equiv (st:boolState) (st':BExpState) (init:state) =
+  fst st = fst st' /\ (forall i. boolEval st init i = bexpEval st' init i)
+
+val state_equiv_impl : st:boolState -> st':BExpState -> init:state -> i:int ->
+  Lemma (requires (state_equiv st st' init))
+        (ensures  (boolEval st init i = bexpEval st' init i))
+let state_equiv_impl st st' init i = ()
+
+val eval_bexp_swap : st:boolState -> st':BExpState -> bexp:BoolExp -> init:state ->
+  Lemma (requires (state_equiv st st' init))
+        (ensures  (evalBexp (substBexp bexp (snd st')) init =
+                   evalBexp bexp (snd st)))
+let rec eval_bexp_swap st st' bexp init = match bexp with
+  | BFalse -> ()
+  | BVar i -> ()
+  | BNot x -> (); eval_bexp_swap st st' x init
+  | BXor (x, y) | BAnd (x, y) -> ();
+    eval_bexp_swap st st' x init;
+    eval_bexp_swap st st' y init
+
+val state_equiv_alloc : st:boolState -> st':BExpState -> init:state -> bexp:BoolExp ->
+  Lemma (requires (state_equiv st st' init))
+        (ensures  (state_equiv (snd (boolAlloc st bexp)) (snd (bexpAlloc st' bexp)) init))
+let state_equiv_alloc st st' init bexp = eval_bexp_swap st st' bexp init
+
+val state_equiv_assign : st:boolState -> st':BExpState -> init:state -> l:int -> bexp:BoolExp ->
+  Lemma (requires (state_equiv st st' init))
+        (ensures  (state_equiv (boolAssign st l bexp) (bexpAssign st' l bexp) init))
+let state_equiv_assign st st' init l bexp = eval_bexp_swap st st' bexp init
+
+val state_equiv_step : gexp:GExpr -> st:boolState -> st':BExpState -> init:state ->
+  Lemma (requires (state_equiv st st' init))
+        (ensures
+          (is_Err (step (gexp, st) boolInterp) /\ is_Err (step (gexp, st') bexpInterp)) \/
+          (is_Val (step (gexp, st) boolInterp) /\ is_Val (step (gexp, st') bexpInterp) /\
+          (fst (getVal (step (gexp, st) boolInterp)) =
+           fst (getVal (step (gexp, st') bexpInterp)) /\
+          state_equiv (snd (getVal (step (gexp, st) boolInterp)))
+                      (snd (getVal (step (gexp, st') bexpInterp)))
+                      init)))
+  (decreases %[gexp;1])
+val state_equiv_step_lst : lst:list GExpr -> st:boolState -> st':BExpState -> init:state ->
+  Lemma (requires (state_equiv st st' init))
+        (ensures
+          (is_Err (step_lst (lst, st) boolInterp) /\ is_Err (step_lst (lst, st') bexpInterp)) \/
+          (is_Val (step_lst (lst, st) boolInterp) /\ is_Val (step_lst (lst, st') bexpInterp) /\
+          (fst (getVal (step_lst (lst, st) boolInterp)) =
+           fst (getVal (step_lst (lst, st') bexpInterp)) /\
+          state_equiv (snd (getVal (step_lst (lst, st) boolInterp)))
+                      (snd (getVal (step_lst (lst, st') bexpInterp)))
+                      init)))
+  (decreases %[lst;0])
+let rec state_equiv_step gexp st st' init = match gexp with
+  | LET (x, t1, t2) ->
+    state_equiv_step t1 st st' init
+  | LAMBDA (x, ty, t) -> ()
+  | APPLY (t1, t2) ->
+    state_equiv_step t1 st st' init;
+    state_equiv_step t2 st st' init
+  | SEQUENCE (t1, t2) ->
+    state_equiv_step t1 st st' init
+  | ASSIGN (t1, t2) ->
+    state_equiv_step t1 st st' init;
+    state_equiv_step t2 st st' init;
+    if (isVal t1 && isBexp t2) then
+      begin match t1 with
+        | LOC l -> state_equiv_assign st st' init l (get_bexp t2)
+        | _ -> ()
+      end
+  | XOR (t1, t2) ->
+    state_equiv_step t1 st st' init;
+    state_equiv_step t2 st st' init
+  | AND (t1, t2) ->
+    state_equiv_step t1 st st' init;
+    state_equiv_step t2 st st' init
+  | BOOL b -> ()
+  | APPEND (t1, t2) ->
+    state_equiv_step t1 st st' init;
+    state_equiv_step t2 st st' init
+  | ROT (i, t) ->
+    state_equiv_step t st st' init
+  | SLICE (t, i, j) ->
+    state_equiv_step t st st' init
+  | ARRAY lst ->
+    state_equiv_step_lst lst st st' init
+  | GET_ARRAY (t, i) ->
+    state_equiv_step t st st' init
+  | ASSERT t ->
+    state_equiv_step t st st' init
+  | BEXP bexp -> state_equiv_alloc st st' init bexp
+  | _ -> ()
+and state_equiv_step_lst lst st st' init = match lst with
+  | [] -> ()
+  | x::xs ->
+    state_equiv_step x st st' init;
+    state_equiv_step_lst xs st st' init
