src/GC.fst
@@ -1,0 +1,141 @@
+(** Garbage collection *)
+module GC
+
+(* Garbage-collected reversible circuit compilation -- experimental *)
+type qubit =
+  { id   : int;
+    ival : BoolExp;
+    cval : BoolExp }
+
+val null_q : qubit
+val get_subst : Total.t int qubit -> int -> Tot int
+val data_q : int -> Tot qubit
+val anc_q  : int -> Tot qubit
+
+let nullq = { id = 0; ival = BFalse; cval = BFalse }
+let get_subst m = fun i -> (m i).id
+let data_q i = { id = i; ival = BVar i; cval = BFalse }
+let anc_q i  = { id = i; ival = BFalse; cval = BFalse }
+
+type circGCState =
+  { top    : int;
+    ah     : AncHeap;
+    gates  : list Gate;
+    symtab : Total.t int qubit }
+
+val circGC       : circGCState -> int -> Tot circGCState
+val circGCInit   : circGCState
+val circGCAlloc  : circGCState -> BoolExp -> Tot (int * circGCState)
+val circGCAssign : circGCState -> int -> BoolExp -> Tot circGCState
+val circGCEval   : circGCState -> state -> int -> Tot bool
+
+// The garbage collector needs to:
+//  -compile the current value in place (i.e. ival + cval + cval = ival),
+//  -if the qubit is an ancilla, push it back onto the heap, and
+//  -update the current value of all other bits by substituting q.id with ival + cval
+val garbageCollect : circGCState -> qubit -> Tot circGCState
+let garbageCollect cs q = 
+  let (ah', res, ancs, circ) = compileBexp cs.ah q.id q.cval in
+  let ah'' = if q.ival = BFalse then insert ah' q.id else ah' in
+  let f q' = 
+    let subq = fun v -> if v = q.id then BXor (q.ival, q.cval) else BVar v in
+      { id = q'.id; ival = q'.ival; cval = simplify (substBexp q'.cval subq) }
+  in
+  let symtab' = mapVal f cs.symtab in
+    { top = cs.top; ah = ah''; gates = cs.gates @ circ; symtab = symtab' }
+
+let circGCInit = { top = 0; ah = emptyHeap; gates = []; subs = constMap nullq;
+symtab = constMap nullq }
+let circGCAlloc cs bexp = 
+  let bexp' = simplify (substVar bexp (get_subst cs.symtab)) in
+  let (ah', bit) = popMin cs.ah in
+  let (ah'', res, ancs, circ') = compileBexp ah' bit bexp' in
+  let q = { id = bit; ival = BFalse; cval = bexp' } in
+  let top' = cs.top + 1 in
+  let gates' = cs.gates @ circ' in
+  let symtab' = update cs.symtab cs.top q in
+  (cs.top, {top = top'; ah = ah''; gates = gates'; symtab = symtab'})
+let circGCAssign cs l bexp =
+  let q = lookup cs.symtab l in
+  let bexp' = simplify (substVar bexp (get_subst cs.symtab)) in
+  let bexpfac = factorAs bexp' q.id in
+  match (q.cval, bexpfac) with
+    | (BFalse, _)      -> // substitute q.id with BFalse, compile in place
+      let bexp'' = substBexp bexp' (fun v -> if v = q.id then BFalse else BVar v) in
+      let (ah', res, ancs, circ) = compileBexp cs.ah q.id bexp'' in
+      let q' = { id = q.id; ival = q.ival; cval = bexp'' } in
+        {top = cs.top; ah = ah'; gates = cs.gates @ circ; symtab = update cs.symtab l q' }
+    | (_, Some bexp'') -> // compile in place, substitute q.id with q.id \oplus bexp''
+      let (ah', res, ancs, circ') = compileBexp cs.ah q.id bexp'' in
+      let q' = { id = q.id; ival = q.ival; cval = simplify (BXor (q.cval, bexp'')) } in
+      let f b = 
+        let subq = fun v -> if v = q.id then BXor (BVar q.id, bexp'') else BVar v in
+          { id = b.id; ival = b.ival; cval = simplify (substBexp b.cval subq) }
+      in
+      let symtab' = update (mapVal f cs.symtab) l q' in
+        {top = cs.top; ah = ah'; gates = cs.gates @ circ'; symtab = update cs.symtab l q' }
+    | _                -> // Compile out of place, clean q.id
+      let (ah', res, ancs, circ') = compileBexp_oop cs.ah bexp' in
+      let q' = { id = res; ival = BFalse; cval = bexp' } in
+      let cs' = { top = cs.top; ah = ah'; gates = cs.gates @ circ'; symtab = update cs.symtab l q' } in
+        garbageCollect cs' q
+let circGCEval cs st i = false
+
+let circGCInterp = {
+  alloc = circGCAlloc;
+  assign = circGCAssign;
+  eval = circGCEval
+}
+
+val allocNcircGC : list GExpr * circGCState -> i:int ->
+  Tot (list GExpr * circGCState) (decreases i)
+let rec allocNcircGC (locs, cs) i =
+  if i <= 0 then (List.rev locs, cs)
+  else
+    let (ah', res) = popMin cs.ah in
+    let cs' = { top = cs.top + 1;
+                ah = ah';
+                gates = cs.gates;
+                symtab = update cs.symtab cs.top (data_q res) }
+    in
+      allocNcircGC (((LOC cs.top)::locs), cs') (i-1)
+
+val allocTycircGC : GType -> circGCState -> Tot (result (GExpr * circGCState))
+let allocTycircGC ty cs = match ty with
+  | GBool ->
+    let (ah', res) = popMin cs.ah in
+    let cs' = { top = cs.top + 1;
+                ah = ah';
+                gates = cs.gates;
+                symtab = update cs.symtab cs.top (data_q res) }
+    in
+      Val (LOC cs.top, cs')
+  | GArray n ->
+    let (locs, st') = allocNcircGC ([], cs) n in
+      Val (ARRAY locs, st')
+  | _ -> Err "Invalid parameter type for circuit generation"
+
+val lookup_Lst_gc : Total.t int qubit -> lst:(list GExpr){isVal_lst lst} -> Tot (list int)
+let rec lookup_Lst_gc symtab lst = match lst with
+  | [] -> []
+  | (LOC l)::xs -> ((lookup symtab l).id)::(lookup_Lst_gc symtab xs)
+
+val compileGCCirc : config circGCState -> Dv (result (list int * list Gate))
+let rec compileGCCirc (gexp, cs) =
+  if isVal gexp then match gexp with
+    | UNIT -> Val ([], [])
+    | LAMBDA (x, ty, t) ->
+      begin match allocTycircGC ty cs with
+        | Err s -> Err s
+        | Val (v, cs') -> compileGCCirc (substGExpr t x v, cs')
+      end
+    | LOC l ->
+      let res = lookup cs.symtab l in
+        Val ([res.id], cs.gates)
+    | ARRAY lst ->
+      let res = lookup_Lst_gc cs.symtab lst in
+        Val (res, cs.gates)
+  else match (step (gexp, cs) circGCInterp) with
+    | Err s -> Err s
+    | Val c' -> compileGCCirc c'
+
